WIP; Universe problems.

theories/MTele.v
@@ -1,55 +1,183 @@
-(** MTele: a telescope which represents functions of the type
-      `X -> ... -> Z -> M R`
-    where R may depend on the value given for X and Y
+From Mtac2 Require Import Sorts.
+Import Sorts.
+
+Set Universe Polymorphism.
+Unset Universe Minimization ToSet.
+
+(** MTele: a telescope which represent nested binder
 
    This will be used to represent legal types of patterns and fixpoints.
+
  *)
 Inductive MTele : Type :=
-| mBase (R : Type) : MTele
+| mBase : MTele
 | mTele {X : Type} (F : X -> MTele) : MTele
 .
 
-Notation "'[tele' x .. y , b ]" := (mTele (fun x => .. (mTele (fun y => mBase b)) .. )) (at level 100, x binder, y binder).
-
-(** MTele_ty: calculate `X -> ... -> Z -> M R` from a given MTele
-
-   To be able to use this in the definition of M.t itself, we paramatrize by M.
-*)
-Fixpoint MTele_ty M (m : MTele) : Prop :=
-  match m with
-  | mBase R => M R
-  | @mTele X F => forall (x : X), MTele_ty M (F x)
+(** MTele_Sort: compute `∀ x .. z, Type` from a given MTele *)
+Fixpoint MTele_Sort (s : Sort) (n : MTele) : Type :=
+  match n with
+  | mBase => s
+  | mTele F => forall x, MTele_Sort s (F x)
   end.
 
-(** Constant MTele_ty *)
-Fixpoint MTele_C (M : Type -> Prop) (b : forall R, M R) m : MTele_ty M m :=
-  match m with
-  | mBase R => b R
-  | mTele F => fun x => MTele_C M b (F x)
+Definition MTele_Ty := (MTele_Sort SType).
+Definition MTele_Pr := (MTele_Sort SProp).
+
+Fixpoint MTele_sort {s : Sort} {n : MTele} :
+  forall S : MTele_Sort s n, Type :=
+  match n return MTele_Sort s n -> Type with
+  | mBase => fun S => selem_of S
+  | mTele F => fun S => forall x, MTele_sort (S x)
   end.
 
+(** Register MTele_ty as a coercion so that we can pretend any `MTele` is a
+    type. *)
+(* Coercion MTele_Ty : MTele >-> Sortclass. *)
 
-Fixpoint MTele_map' (M : Type -> Prop) {X : forall R :Type, Prop} (m : MTele) : forall (f : MTele_ty (fun R => M R -> X R) m), MTele_ty M m -> MTele_ty (fun R => X R) m :=
-  match m as m' return _ m' -> MTele_ty M m' -> MTele_ty _ m' with
-  | mBase R => fun (f : M R -> X R) (t : M R) => f t
-  | mTele F => fun (f : forall x : _, MTele_ty _ (F x)) (t : forall x : _, MTele_ty M (F x)) =>
-                 fun x : _ => MTele_map' M (F x) (f x) (t x)
+(** MTele_val: compute `λ x .. z, T x .. z` from `T : MTele_ty n` *)
+Definition MTele_val {s} : forall {n : MTele}, MTele_Sort s n -> s :=
+  fix go n :=
+    match n as n return MTele_Sort s n -> s with
+    | mBase => fun f => f
+    | mTele F => fun f => ForAll (fun x => go _ (f x))
+    end.
+
+Definition MTele_valT {n} : MTele_Ty n -> Type :=
+  MTele_val (s := SType) (n:=n).
+  (* ltac:( *)
+  (*   let e := constr:(MTele_val (s := SType) (n:=n)) in *)
+  (*   let e := (eval red in e) in *)
+  (*   let e := (eval cbv match beta delta [ForAll stype_of] in e) in *)
+  (*   let e := (eval fold MTele_Ty in e) in *)
+  (*   exact e). *)
+Definition MTele_valP {n} : MTele_Pr n -> Prop :=
+  MTele_val (s := SProp) (n:=n).
+
+(* Coercion MTele_valT : MTele_Ty >-> Sortclass. *)
+
+(** MTele_In: gain access to potentially multiple telescoped types and values at
+the same time to compute a new telescoped _type_. *)
+Fixpoint MTele_In (s : Sort) {n : MTele} :
+  (forall (now_ty : forall s, MTele_Sort s n -> s)
+          (now_val : forall s {T : MTele_Sort s n}, MTele_val T -> now_ty s T), s)
+  -> MTele_Sort s n :=
+  match n as n return
+        (forall (now_ty : forall s, MTele_Sort s n -> s)
+                (now_val : forall s {T : MTele_Sort s n}, MTele_val T -> now_ty s T), s)
+        -> MTele_Sort s n
+  with
+  | mBase => fun thunk => thunk (fun s T => T) (fun _ _ v => v)
+  | mTele F =>
+    fun thunk t =>
+      MTele_In s (fun now_ty now_val =>
+                    thunk
+                      (fun _ T => now_ty _ (T t))
+                      (fun _ _ v => now_val _ _ (App v t))
+                 )
   end.
 
-Fixpoint MTele_mkfunc (M : Type -> Prop) {X : Type -> Prop} (b : forall R, M R -> X R) (m : MTele) : MTele_ty (fun R => M R -> X R) m :=
-  match m as m' return MTele_ty (fun R => M R -> X R) m' with
-  | mBase R => fun t => b _ t
-  | mTele F => fun x => MTele_mkfunc M b (F x)
+Notation "'[WithT' now_ty , now_val '=>' T ]" :=
+  (MTele_In SType (fun now_ty now_val => T))
+    (at level 0, format "[WithT  now_ty ,  now_val  =>  T ]").
+
+(** MTele_in: gain access to potentially multiple telescoped types and values at the same time to compute a new telescoped _value_ of type `MTele_In ..`. *)
+Fixpoint MTele_in (s : Sort) {n : MTele} :
+  forall {thunk},
+  (forall (now_ty : forall s, MTele_Sort s n -> s)
+          (now_val : forall s {T : MTele_Sort s n}, MTele_val T -> now_ty s T),
+      now_ty s (MTele_In s thunk))
+  -> MTele_val (MTele_In (n:=n) s thunk) :=
+  match n as n return
+        forall thunk,
+        (forall (now_ty : forall s, MTele_Sort s n -> s)
+                (now_val : forall s {T : MTele_Sort s n}, MTele_val T -> now_ty s T),
+            now_ty s (MTele_In s thunk)
+        )
+        -> MTele_val (MTele_In (n:=n) s thunk)
+  with
+  | mBase => fun _ thunk => thunk (fun s T => T) (fun _ _ v => v)
+  | mTele F =>
+    fun _ thunk =>
+      Fun (fun t =>
+             MTele_in s (fun now_ty now_val =>
+                           thunk
+                             (fun _ T => now_ty _ (T t))
+                             (fun _ _ v => now_val _ _ (App v t))
+                        )
+          )
   end.
 
-Notation MT_Acc R m := (forall (M' : Type -> Prop), MTele_ty M' m -> M' R).
+Notation "'[withT' now_ty , now_val '=>' t ]" :=
+  (MTele_in (SType) (fun now_ty now_val => t))
+    (at level 0, format "[withT  now_ty ,  now_val  =>  t ]").
 
-Fixpoint MTele_open (M : Type -> Prop) {X : Type -> Prop} m :
-  (forall R, MT_Acc R m -> X R) -> MTele_ty X m  :=
-  match m as m' return (forall R, MT_Acc R m' -> X R) -> MTele_ty X m' with
-  | mBase R => fun b => b R (fun M' x => x)
-  | mTele F => fun b x => MTele_open M (F x) (fun R f => b R (fun M' mR => f M' (mR x)))
+(** MTele_Map: compute type `∀ x .. z, B x .. z` from type
+    `∀ x .. z, A x .. z` *)
+Fixpoint MTele_Map (s so : Sort) {n : MTele} :
+  MTele_sort (MTele_In (SType) (n := n) (fun _ _ => stype_of s -> stype_of so)) -> MTele_Sort s n -> MTele_Sort so n
+  :=
+  match n return
+        MTele_sort (MTele_In (SType) (n := n) (fun _ _ => stype_of s -> stype_of so)) -> MTele_Sort s n -> MTele_Sort so n
+  with
+  | mBase => fun f A => f A
+  | mTele F => fun f A t => @MTele_Map s so (F t) (f t) (A t)
   end.
 
-Definition MTele_map (M : Type -> Prop) {X : Type -> Prop}  (b : forall R, M R -> X R) (m : MTele) : MTele_ty M m -> MTele_ty (fun R => X R) m :=
-  MTele_map' M _ (MTele_mkfunc _ b m).
+(** MTele_C: MTele_map with a constant function *)
+Fixpoint MTele_C (s so : Sort) {n : MTele} :
+  (s -> so) -> MTele_Sort s n -> MTele_Sort so n :=
+  match n return (s -> so) -> MTele_Sort s n -> MTele_Sort so n with
+  | mBase => fun f A => f A
+  | mTele F => fun f A t => MTele_C s so f (A t)
+  end.
+
+Fixpoint MTele_c (s so : Sort) {n : MTele} :
+  forall (G : s -> so)
+         (g : ForAll G)
+         (T : MTele_Sort s n),
+  MTele_val T -> MTele_val (MTele_C _ _ G T) :=
+  match n with
+  | mBase => fun G g T v => App g _
+  | mTele F => fun G g T v => Fun (fun x => MTele_c s so G g (T x) (App v x))
+  end.
+
+(* MTele_map: map values of type `∀ x .. z, A x .. z` to values of type
+   `∀ x .. z, B x .. z` *)
+Fixpoint MTele_map {s} {n : MTele} :
+  forall {A : MTele_Sort s n} {B :  MTele_Sort s n},
+    MTele_val (MTele_In s (fun ty _ => Impl (ty _ A) (ty _ B))) -> MTele_val A -> MTele_val B :=
+  match n with
+  | mBase => fun A B f a => App f a
+  | mTele F => fun A B f a => Fun (fun t => MTele_map (App f t) (App a t))
+  end.
+
+(** MTele_id: a sanity check to see if we can witness `(∀ x .. z, A x .. z) ->
+(∀ x .. z, A x .. z)` by constructing `∀ x .. z, A x .. z -> A x .. z` *)
+Local Fixpoint MTele_id {s} (n : MTele) :
+  forall {A : MTele_Sort s n},
+    MTele_val (MTele_In s (fun ty _ => Impl (ty _ A) (ty _ A))) :=
+  match n  with
+  | mBase => fun A => Fun (fun x : selem_of A => x)
+  | mTele F => fun A => Fun (fun x => MTele_id (F x))
+  end.
+
+Local Example map_id {s} {n : MTele} {A : MTele_Sort s n} := @MTele_map s n A A (MTele_id n).
+
+
+(* Old MTele functions redefined on top of the more general newer ones above *)
+
+Definition MTele_ty (M : Type -> Prop) {n : MTele} :
+  forall A : MTele_Ty n, Prop :=
+  fun A => MTele_val (MTele_C SType SProp M A).
+
+Notation MT_Acc R T := (forall (M' : Type -> Prop), MTele_ty M' T -> M' R).
+
+(* MTele_open: old telescope accessor *)
+Fixpoint MTele_open (M : Type -> Prop) {X : Type -> Prop} {m}:
+  forall (T : MTele_Ty m),
+    (forall R, MT_Acc R T -> X R) -> MTele_ty X T  :=
+  match m as m' return forall T : MTele_Ty m', (forall R, MT_Acc R T -> X R) -> MTele_ty X T with
+  | mBase => fun T b => b _ (fun X x => x)
+  | mTele F => fun T b x => MTele_open M (T x) (fun R f => b R (fun M' mR => f M' (mR x)))
+  end.
